wip on parsing boogie goal

ParseSMT.v
@@ -1,25 +1,158 @@
 Require Import Coq.ZArith.ZArith. Open Scope Z_scope.
+Require Import Coq.Lists.List. Import ListNotations.
 Require Import Coq.micromega.Lia.
 
+Definition allDistinct{A: Type}(l: list A): Prop :=
+  forall i j e1 e2, nth_error l i = Some e1 -> nth_error l j = Some e2 -> e1 = e2 -> i = j.
+
 (* Structure *)
+
 Notation "'(check-sat)'" := False (only parsing).
 Notation "'(assert' P ')' Q" := (P -> Q) (only parsing, at level 10).
+
 Notation "'(declare-fun' f '()' T ')' Q" := (forall (f: T), Q)
-  (only parsing, at level 10, T at level 0, Q at level 0).
+  (only parsing, at level 10, f at level 0, T at level 200, Q at level 0).
+Notation "'(declare-fun' f '(' A1 ')' T ')' Q" := (forall (f: A1 -> T), Q)
+  (only parsing, at level 10, f at level 0, T at level 0, Q at level 0, A1 at level 0).
+Notation "'(declare-fun' f '(' A1 A2 ')' T ')' Q" := (forall (f: A1 -> A2 -> T), Q)
+  (only parsing, at level 10, f at level 0, T at level 0, Q at level 0,
+   A1 at level 0, A2 at level 0).
+Notation "'(declare-fun' f '(' A1 A2 A3 ')' T ')' Q" := (forall (f: A1 -> A2 -> A3 -> T), Q)
+  (only parsing, at level 10, f at level 0, T at level 0, Q at level 0,
+   A1 at level 0, A2 at level 0, A3 at level 0).
+Notation "'(declare-fun' f '(' A1 A2 A3 A4 ')' T ')' Q" :=
+  (forall (f: A1 -> A2 -> A3 -> A4 -> T), Q)
+  (only parsing, at level 10, f at level 0, T at level 0, Q at level 0,
+   A1 at level 0, A2 at level 0, A3 at level 0, A4 at level 0).
+
 (* TODO a recursive notation over nat could also support "Type -> Type -> Type -> ..." etc *)
 Notation "'(declare-sort' T '0' ')' Q" := (forall (T: Type), Q)
   (only parsing, at level 10, Q at level 0, T at level 0).
 
+Notation "'(forall' '(' '(' x1 T1 ')' ')' P ')'" :=
+  ( forall (x1: T1), P)
+  (only parsing, at level 0, x1 at level 0, T1 at level 0,
+   P at level 0).
+(*
+Notation "'(forall' '(' '(' x1 T1 ')' ')' '(!' P ':pattern' '(' pat1 ')' ')' ')'" :=
+  ( forall x1: T1, P)
+  (only parsing, at level 10, x1 at level 0, T1 at level 0,
+   P at level 0, pat1 at level 0).
+
+
+Notation "'(forall' '(' '(' x1 T1 ')' '(' x2 T2 ')' ')' '(!' P ':pattern' '(' pat1 pat2 ')' ')' ')'" :=
+  ( forall (x1: T1) (x2: T2), P)
+  (only parsing, at level 10, x1 at level 0, T1 at level 0, x2 at level 0, T2 at level 0,
+   P at level 0, pat1 at level 0, pat2 at level 0).
+*)
+
+Notation "'(forall' '(' '(' x1 T1 ')' '(' x2 T2 ')' ')' P ')'" :=
+  ( forall (x1: T1) (x2: T2), P)
+  (only parsing, at level 0, x1 at level 0, T1 at level 0, x2 at level 0, T2 at level 0,
+   P at level 0).
+Notation "'(forall' '(' '(' x1 T1 ')' '(' x2 T2 ')' '(' x3 T3 ')' ')' P ')'" :=
+  ( forall (x1: T1) (x2: T2) (x3: T3), P)
+    (only parsing, at level 0,
+     x1 at level 0, T1 at level 0,
+     x2 at level 0, T2 at level 0,
+     x3 at level 0, T3 at level 0,
+   P at level 0).
+Notation "'(forall' '(' '(' x1 T1 ')' '(' x2 T2 ')' '(' x3 T3 ')' '(' x4 T4 ')' ')' P ')'" :=
+  ( forall (x1: T1) (x2: T2) (x3: T3) (x4: T4), P)
+    (only parsing, at level 0,
+     x1 at level 0, T1 at level 0,
+     x2 at level 0, T2 at level 0,
+     x3 at level 0, T3 at level 0,
+     x4 at level 0, T4 at level 0,
+   P at level 0).
+Notation "'(forall' '(' '(' x1 T1 ')' '(' x2 T2 ')' '(' x3 T3 ')' '(' x4 T4 ')' '(' x5 T5 ')' ')' P ')'" :=
+  ( forall (x1: T1) (x2: T2) (x3: T3) (x4: T4) (x5: T5), P)
+    (only parsing, at level 0,
+     x1 at level 0, T1 at level 0,
+     x2 at level 0, T2 at level 0,
+     x3 at level 0, T3 at level 0,
+     x4 at level 0, T4 at level 0,
+     x5 at level 0, T5 at level 0,
+   P at level 0).
+Notation "'(forall' '(' '(' x1 T1 ')' '(' x2 T2 ')' '(' x3 T3 ')' '(' x4 T4 ')' '(' x5 T5 ')' '(' x6 T6 ')' ')' P ')'" :=
+  ( forall (x1: T1) (x2: T2) (x3: T3) (x4: T4) (x5: T5) (x6: T6), P)
+    (only parsing, at level 0,
+     x1 at level 0, T1 at level 0,
+     x2 at level 0, T2 at level 0,
+     x3 at level 0, T3 at level 0,
+     x4 at level 0, T4 at level 0,
+     x5 at level 0, T5 at level 0,
+     x6 at level 0, T6 at level 0,
+   P at level 0).
+
+Notation "'(let' '(' '(' v1 t1 ')' ')' u ')'" :=
+  (let v1 := t1 in u)
+    (only parsing, at level 0,
+     v1 at level 0, t1 at level 0,
+     u at level 0).
+Notation "'(let' '(' '(' v1 t1 ')' '(' v2 t2 ')' ')' u ')'" :=
+  ( let v1 := t1 in let v2 := t2 in u)
+    (only parsing, at level 0,
+     v1 at level 0, t1 at level 0,
+     v2 at level 0, t2 at level 0,
+     u at level 0).
+Notation "'(let' '(' '(' v1 t1 ')' '(' v2 t2 ')' '(' v3 t3 ')' ')' u ')'" :=
+  ( let v1 := t1 in let v2 := t2 in let v3 := t3 in u)
+    (only parsing, at level 0,
+     v1 at level 0, t1 at level 0,
+     v2 at level 0, t2 at level 0,
+     v3 at level 0, t3 at level 0,
+     u at level 0).
+
+
+(* ignores the pattern *)
+Definition with_pattern{P T: Type}(pat: P)(t: T): T := t.
+
+Notation "'(!' P ':pattern' '(' x y .. z ')' ')'" :=
+  (with_pattern x (with_pattern y .. (with_pattern z P) .. ))
+  (only parsing, at level 0, x at level 0).
+
+Notation "'(!' P ':pattern' '(' x ')' ')'" :=
+  (with_pattern x P)
+  (only parsing, at level 0, x at level 0).
+
+(*
+(assert (forall ((c0 Int) (c1 Int)) (! (=> (not (= c0 c1)) (not (= (ClassRepr c0) (ClassRepr c1)))) :pattern ((ClassRepr c0) (ClassRepr c1)) )))
+*)
 
 (* Operations *)
 Notation "'(<=' a b ')'" := (a <= b) (only parsing, a at level 0, b at level 0).
+Notation "'(<' a b ')'" := (a < b) (only parsing, a at level 0, b at level 0).
 Notation "'(=' a b ')'" := (a = b) (only parsing, a at level 0, b at level 0).
 Notation "'(+' a b ')'" := (a + b) (only parsing, a at level 0, b at level 0).
+Notation "'(-' a b ')'" := (a - b) (only parsing, a at level 0, b at level 0).
 (* Note: if we omit the space, it becomes a Coq comment! *)
 Notation "'(' '*' a b ')'" := (a * b) (only parsing, a at level 0, b at level 0).
 
+(* Logic operators *)
+Notation "'(=>' a b ')'" := (a -> b) (only parsing, a at level 0, b at level 0).
+Notation "'(and' a b ')'" := (a /\ b) (only parsing, a at level 0, b at level 0).
+Notation "'(and' a b c ')'" := (a /\ b /\ c) (only parsing, a at level 0, b at level 0, c at level 0).
+Notation "'(and' a b c d ')'" := (a /\ b /\ c /\ d) (only parsing, a at level 0, b at level 0, c at level 0, d at level 0).
+Notation "'(and' a b c d e ')'" := (a /\ b /\ c /\ d /\ e) (only parsing, a at level 0, b at level 0, c at level 0, d at level 0, e at level 0).
+Notation "'(and' a b c d e f ')'" := (a /\ b /\ c /\ d /\ e /\ f) (only parsing, a at level 0, b at level 0, c at level 0, d at level 0, e at level 0, f at level 0).
+Notation "'(or' a b ')'" := (a \/ b) (only parsing, a at level 0, b at level 0).
+Notation "'(not' a ')'" := (~ a) (only parsing, a at level 0).
+
+(* Misc logic hack *)
+Notation "'(=' a 'true)'" := (a: Prop) (only parsing, a at level 0).
+
 (* Datatypes *)
 Notation Int := Z (only parsing).
+Notation Bool := Prop (only parsing). (* TODO sometimes "bool" might be more appropriate *)
+
+(* Misc *)
+Notation "'(distinct' x y .. z ')'" := (allDistinct (cons x (cons y .. (cons z nil) ..)))
+  (only parsing, at level 10, x at level 0, y at level 0, z at level 0).
+(*
+coq/theories/Lists/List.v:
+Notation "[ x ; y ; .. ; z ]" :=  (cons x (cons y .. (cons z nil) ..)) : list_scope.
+*)
 
 Goal
   (* from https://www.starexec.org/starexec/secure/details/benchmark.jsp?id=7239749 *)
@@ -38,11 +171,409 @@ Proof.
   lia.
 Qed.
 
+Goal
+(*
+UFLIA example from boogie from SMT competition
+https://www.starexec.org/starexec/services/benchmarks/7158337/contents?limit=-1
+preprocessed with preprocess.sh
+*)
+(declare-fun boolIff (Int Int) Int)
+(declare-fun PeerGroupPlaceholder_ () Int)
+(declare-fun intGreater (Int Int) Int)
+(declare-fun IfThenElse_ (Int Int Int) Int)
+(declare-fun CONCVARSYM (Int) Int)
+(declare-fun SharingMode_Unshared_ () Int)
+(declare-fun System_dot_Reflection_dot_IReflect () Int)
+(declare-fun int_m2147483648 () Int)
+(declare-fun System_dot_Int32 () Int)
+(declare-fun intAtMost (Int Int) Int)
+(declare-fun multiply (Int Int) Int)
+(declare-fun Is_ (Int Int) Int)
+(declare-fun Smt_dot_true () Int)
+(declare-fun Bag () Int)
+(declare-fun ElementType_ (Int) Int)
+(declare-fun divide (Int Int) Int)
+(declare-fun int_m9223372036854775808 () Int)
+(declare-fun divides (Int Int) Int)
+(declare-fun select1 (Int Int) Int)
+(declare-fun store1 (Int Int Int) Int)
+(declare-fun select2 (Int Int Int) Int)
+(declare-fun nullObject () Int)
+(declare-fun store2 (Int Int Int Int) Int)
+(declare-fun modulo (Int Int) Int)
+(declare-fun ownerRef_ () Int)
+(declare-fun StructSet_ (Int Int Int) Int)
+(declare-fun AsDirectSubClass (Int Int) Int)
+(declare-fun System_dot_Collections_dot_ICollection () Int)
+(declare-fun System_dot_Boolean () Int)
+(declare-fun shl_ (Int Int) Int)
+(declare-fun DimLength_ (Int Int) Int)
+(declare-fun anyEqual (Int Int) Int)
+(declare-fun System_dot_Array () Int)
+(declare-fun System_dot_Reflection_dot_ICustomAttributeProvider () Int)
+(declare-fun SharingMode_LockProtected_ () Int)
+(declare-fun IsMemberlessType_ (Int) Int)
+(declare-fun System_dot_UInt16 () Int)
+(declare-fun ClassRepr (Int) Int)
+(declare-fun System_dot_Runtime_dot_InteropServices_dot__Type () Int)
+(declare-fun boolNot (Int) Int)
+(declare-fun Microsoft_dot_Contracts_dot_ICheckedException () Int)
+(declare-fun System_dot_Exception () Int)
+(declare-fun System_dot_Runtime_dot_InteropServices_dot__MemberInfo () Int)
+(declare-fun block6086_correct () Int)
+(declare-fun boolAnd (Int Int) Int)
+(declare-fun boolImplies (Int Int) Int)
+(declare-fun Unbox (Int) Int)
+(declare-fun intAtLeast (Int Int) Int)
+(declare-fun ownerFrame_ () Int)
+(declare-fun int_4294967295 () Int)
+(declare-fun IsAllocated (Int Int) Int)
+(declare-fun TypeName (Int) Int)
+(declare-fun AsPeerField (Int) Int)
+(declare-fun int_9223372036854775807 () Int)
+(declare-fun AsRepField (Int Int) Int)
+(declare-fun System_dot_Reflection_dot_MemberInfo () Int)
+(declare-fun ArrayCategoryValue_ () Int)
+(declare-fun is (Int Int) Int)
+(declare-fun Microsoft_dot_Contracts_dot_GuardException () Int)
+(declare-fun InRange (Int Int) Bool)
+(declare-fun AsOwner (Int Int) Int)
+(declare-fun System_dot_Int64 () Int)
+(declare-fun System_dot_Runtime_dot_InteropServices_dot__Exception () Int)
+(declare-fun or_ (Int Int) Int)
+(declare-fun As_ (Int Int) Int)
+(declare-fun exposeVersion_ () Int)
+(declare-fun System_dot_Type () Int)
+(declare-fun intLess (Int Int) Int)
+(declare-fun AsImmutable_ (Int) Int)
+(declare-fun NonNullFieldsAreInitialized_ () Int)
+(declare-fun LBound_ (Int Int) Int)
+(declare-fun System_dot_Object () Int)
+(declare-fun Bag_dot_a () Int)
+(declare-fun System_dot_UInt32 () Int)
+(declare-fun localinv_ () Int)
+(declare-fun inv_ () Int)
+(declare-fun Bag_dot_n () Int)
+(declare-fun entry_correct () Int)
+(declare-fun FirstConsistentOwner_ () Int)
+(declare-fun UnboxedType (Int) Int)
+(declare-fun AsRefField (Int Int) Int)
+(declare-fun System_dot_Byte () Int)
+(declare-fun int_2147483647 () Int)
+(declare-fun ArrayCategoryRef_ () Int)
+(declare-fun Heap_ () Int)
+(declare-fun Length_ (Int) Int)
+(declare-fun System_dot_Runtime_dot_Serialization_dot_ISerializable () Int)
+(declare-fun AsNonNullRefField (Int Int) Int)
+(declare-fun IsHeap (Int) Int)
+(declare-fun UBound_ (Int Int) Int)
+(declare-fun System_dot_String () Int)
+(declare-fun System_dot_Collections_dot_IList () Int)
+(declare-fun System_dot_String_dot_IsInterned_System_dot_String_notnull_ (Int) Int)
+(declare-fun Rank_ (Int) Int)
+(declare-fun UnknownRef_ () Int)
+(declare-fun RefArraySet (Int Int Int) Int)
+(declare-fun ValueArraySet (Int Int Int) Int)
+(declare-fun boolOr (Int Int) Int)
+(declare-fun sharingMode_ () Int)
+(declare-fun subtypes (Int Int) Bool)
+(declare-fun System_dot_String_dot_Equals_System_dot_String_System_dot_String_ (Int Int) Int)
+(declare-fun anyNeq (Int Int) Int)
+(declare-fun IsStaticField (Int) Int)
+(declare-fun IsNotNull_ (Int Int) Int)
+(declare-fun typeof_ (Int) Int)
+(declare-fun ArrayCategoryNonNullRef_ () Int)
+(declare-fun RefArrayGet (Int Int) Int)
+(declare-fun ValueArrayGet (Int Int) Int)
+(declare-fun TypeObject (Int) Int)
+(declare-fun and_ (Int Int) Int)
+(declare-fun BoxTester (Int Int) Int)
+(declare-fun Microsoft_dot_Contracts_dot_ObjectInvariantException () Int)
+(declare-fun IsValueType_ (Int) Int)
+(declare-fun AsRangeField (Int Int) Int)
+(declare-fun System_dot_SByte () Int)
+(declare-fun BeingConstructed_ () Int)
+(declare-fun FieldDependsOnFCO_ (Int Int Int) Int)
+(declare-fun NonNullRefArray (Int Int) Int)
+(declare-fun RefArray (Int Int) Int)
+(declare-fun ArrayCategory_ (Int) Int)
+(declare-fun AsPureObject_ (Int) Int)
+(declare-fun System_dot_String_dot_Equals_System_dot_String_ (Int Int) Int)
+(declare-fun System_dot_Int16 () Int)
+(declare-fun AsMutable_ (Int) Int)
+(declare-fun System_dot_Char () Int)
+(declare-fun block6069_correct () Int)
+(declare-fun System_dot_UInt64 () Int)
+(declare-fun StructGet_ (Int Int) Int)
+(declare-fun OneClassDown (Int Int) Int)
+(declare-fun ArrayIndex (Int Int Int Int) Int)
+(declare-fun Box (Int Int) Int)
+(declare-fun int_18446744073709551615 () Int)
+(declare-fun shr_ (Int Int) Int)
+(declare-fun System_dot_ICloneable () Int)
+(declare-fun IsDirectlyModifiableField (Int) Int)
+(declare-fun StringLength_ (Int) Int)
+(declare-fun allocated_ () Int)
+(declare-fun BaseClass_ (Int) Int)
+(declare-fun ValueArray (Int Int) Int)
+(declare-fun Smt_dot_false () Int)
+(declare-fun IsImmutable_ (Int) Int)
+(declare-fun elements_ () Int)
+(declare-fun DeclType (Int) Int)
+(declare-fun System_dot_Collections_dot_IEnumerable () Int)
+(declare-fun ReallyLastGeneratedExit_correct () Int)
+(assert (distinct allocated_ elements_ inv_ localinv_ exposeVersion_ sharingMode_ SharingMode_Unshared_ SharingMode_LockProtected_ ownerRef_ ownerFrame_ PeerGroupPlaceholder_ ArrayCategoryValue_ ArrayCategoryRef_ ArrayCategoryNonNullRef_ System_dot_Array System_dot_Object System_dot_Type BeingConstructed_ NonNullFieldsAreInitialized_ System_dot_String FirstConsistentOwner_ System_dot_SByte System_dot_Byte System_dot_Int16 System_dot_UInt16 System_dot_Int32 System_dot_UInt32 System_dot_Int64 System_dot_UInt64 System_dot_Char int_m2147483648 int_2147483647 int_4294967295 int_m9223372036854775808 int_9223372036854775807 int_18446744073709551615 UnknownRef_ Bag_dot_a Bag_dot_n Microsoft_dot_Contracts_dot_ObjectInvariantException System_dot_Collections_dot_IEnumerable System_dot_Boolean System_dot_ICloneable System_dot_Reflection_dot_ICustomAttributeProvider System_dot_Runtime_dot_Serialization_dot_ISerializable System_dot_Exception System_dot_Reflection_dot_IReflect System_dot_Runtime_dot_InteropServices_dot__Exception System_dot_Collections_dot_ICollection Microsoft_dot_Contracts_dot_ICheckedException Bag Microsoft_dot_Contracts_dot_GuardException System_dot_Runtime_dot_InteropServices_dot__MemberInfo System_dot_Collections_dot_IList System_dot_Runtime_dot_InteropServices_dot__Type System_dot_Reflection_dot_MemberInfo))
+(assert (= (DeclType exposeVersion_) System_dot_Object))
+(assert (forall ((c0 Int) (c1 Int)) (! (=> (not (= c0 c1)) (not (= (ClassRepr c0) (ClassRepr c1)))) :pattern ((ClassRepr c0) (ClassRepr c1)) )))
+(assert (forall ((T Int)) (not (subtypes (typeof_ (ClassRepr T)) System_dot_Object))))
+(assert (forall ((T Int)) (not (= (ClassRepr T) nullObject))))
+(assert (forall ((T Int) (h Int)) (! (=> (= (IsHeap h) Smt_dot_true) (= (select2 h (ClassRepr T) ownerFrame_) PeerGroupPlaceholder_)) :pattern ((select2 h (ClassRepr T) ownerFrame_)) )))
+(assert (not (= (IsDirectlyModifiableField allocated_) Smt_dot_true)))
+(assert (= (IsDirectlyModifiableField elements_) Smt_dot_true))
+(assert (not (= (IsDirectlyModifiableField inv_) Smt_dot_true)))
+(assert (not (= (IsDirectlyModifiableField localinv_) Smt_dot_true)))
+(assert (not (= (IsDirectlyModifiableField ownerRef_) Smt_dot_true)))
+(assert (not (= (IsDirectlyModifiableField ownerFrame_) Smt_dot_true)))
+(assert (not (= (IsDirectlyModifiableField exposeVersion_) Smt_dot_true)))
+(assert (not (= (IsStaticField allocated_) Smt_dot_true)))
+(assert (not (= (IsStaticField elements_) Smt_dot_true)))
+(assert (not (= (IsStaticField inv_) Smt_dot_true)))
+(assert (not (= (IsStaticField localinv_) Smt_dot_true)))
+(assert (not (= (IsStaticField exposeVersion_) Smt_dot_true)))
+(assert (forall ((A Int) (i Int) (x Int)) (= (ValueArrayGet (ValueArraySet A i x) i) x)))
+(assert (forall ((A Int) (i Int) (j Int) (x Int)) (=> (not (= i j)) (= (ValueArrayGet (ValueArraySet A i x) j) (ValueArrayGet A j)))))
+(assert (forall ((A Int) (i Int) (x Int)) (= (RefArrayGet (RefArraySet A i x) i) x)))
+(assert (forall ((A Int) (i Int) (j Int) (x Int)) (=> (not (= i j)) (= (RefArrayGet (RefArraySet A i x) j) (RefArrayGet A j)))))
+(assert (forall ((a Int) (d Int) (x Int) (y Int) (_x'_ Int) (_y'_ Int)) (! (=> (= (ArrayIndex a d x y) (ArrayIndex a d _x'_ _y'_)) (and (= x _x'_) (= y _y'_))) :pattern ((ArrayIndex a d x y) (ArrayIndex a d _x'_ _y'_)) )))
+(assert (forall ((a Int) (T Int) (i Int) (r Int) (heap Int)) (! (=> (and (= (IsHeap heap) Smt_dot_true) (subtypes (typeof_ a) (RefArray T r))) (= (Is_ (RefArrayGet (select2 heap a elements_) i) T) Smt_dot_true)) :pattern ((subtypes (typeof_ a) (RefArray T r)) (RefArrayGet (select2 heap a elements_) i)) )))
+(assert (forall ((a Int) (T Int) (i Int) (r Int) (heap Int)) (! (=> (and (= (IsHeap heap) Smt_dot_true) (subtypes (typeof_ a) (NonNullRefArray T r))) (= (IsNotNull_ (RefArrayGet (select2 heap a elements_) i) T) Smt_dot_true)) :pattern ((subtypes (typeof_ a) (NonNullRefArray T r)) (RefArrayGet (select2 heap a elements_) i)) )))
+(assert (forall ((a Int)) (<= 1 (Rank_ a))))
+(assert (forall ((a Int) (T Int) (r Int)) (! (=> (and (not (= a nullObject)) (subtypes (typeof_ a) (RefArray T r))) (= (Rank_ a) r)) :pattern ((subtypes (typeof_ a) (RefArray T r))) )))
+(assert (forall ((a Int) (T Int) (r Int)) (! (=> (and (not (= a nullObject)) (subtypes (typeof_ a) (NonNullRefArray T r))) (= (Rank_ a) r)) :pattern ((subtypes (typeof_ a) (NonNullRefArray T r))) )))
+(assert (forall ((a Int) (T Int) (r Int)) (! (=> (and (not (= a nullObject)) (subtypes (typeof_ a) (ValueArray T r))) (= (Rank_ a) r)) :pattern ((subtypes (typeof_ a) (ValueArray T r))) )))
+(assert (forall ((a Int)) (! (<= 0 (Length_ a)) :pattern ((Length_ a)) )))
+(assert (forall ((a Int) (i Int)) (<= 0 (DimLength_ a i))))
+(assert (forall ((a Int)) (! (=> (= (Rank_ a) 1) (= (DimLength_ a 0) (Length_ a))) :pattern ((DimLength_ a 0)) )))
+(assert (forall ((a Int) (i Int)) (! (= (LBound_ a i) 0) :pattern ((LBound_ a i)) )))
+(assert (forall ((a Int) (i Int)) (! (= (UBound_ a i) (- (DimLength_ a i) 1)) :pattern ((UBound_ a i)) )))
+(assert (forall ((T Int) (ET Int) (r Int)) (! (=> (subtypes T (ValueArray ET r)) (= (ArrayCategory_ T) ArrayCategoryValue_)) :pattern ((subtypes T (ValueArray ET r))) )))
+(assert (forall ((T Int) (ET Int) (r Int)) (! (=> (subtypes T (RefArray ET r)) (= (ArrayCategory_ T) ArrayCategoryRef_)) :pattern ((subtypes T (RefArray ET r))) )))
+(assert (forall ((T Int) (ET Int) (r Int)) (! (=> (subtypes T (NonNullRefArray ET r)) (= (ArrayCategory_ T) ArrayCategoryNonNullRef_)) :pattern ((subtypes T (NonNullRefArray ET r))) )))
+(assert (subtypes System_dot_Array System_dot_Object))
+(assert (forall ((T Int) (r Int)) (! (subtypes (ValueArray T r) System_dot_Array) :pattern ((ValueArray T r)) )))
+(assert (forall ((T Int) (r Int)) (! (subtypes (RefArray T r) System_dot_Array) :pattern ((RefArray T r)) )))
+(assert (forall ((T Int) (r Int)) (! (subtypes (NonNullRefArray T r) System_dot_Array) :pattern ((NonNullRefArray T r)) )))
+(assert (forall ((T Int) (U Int) (r Int)) (=> (subtypes U T) (subtypes (RefArray U r) (RefArray T r)))))
+(assert (forall ((T Int) (U Int) (r Int)) (=> (subtypes U T) (subtypes (NonNullRefArray U r) (NonNullRefArray T r)))))
+(assert (forall ((A Int) (r Int)) (= (ElementType_ (ValueArray A r)) A)))
+(assert (forall ((A Int) (r Int)) (= (ElementType_ (RefArray A r)) A)))
+(assert (forall ((A Int) (r Int)) (= (ElementType_ (NonNullRefArray A r)) A)))
+(assert (forall ((A Int) (r Int) (T Int)) (! (let ((v_0 (ElementType_ T))) (=> (subtypes T (RefArray A r)) (and (= T (RefArray v_0 r)) (subtypes v_0 A)))) :pattern ((subtypes T (RefArray A r))) )))
+(assert (forall ((A Int) (r Int) (T Int)) (! (let ((v_0 (ElementType_ T))) (=> (subtypes T (NonNullRefArray A r)) (and (= T (NonNullRefArray v_0 r)) (subtypes v_0 A)))) :pattern ((subtypes T (NonNullRefArray A r))) )))
+(assert (forall ((A Int) (r Int) (T Int)) (let ((v_0 (ValueArray A r))) (=> (subtypes T v_0) (= T v_0)))))
+(assert (forall ((A Int) (r Int) (T Int)) (let ((v_0 (ElementType_ T))) (=> (subtypes (RefArray A r) T) (or (subtypes System_dot_Array T) (and (= T (RefArray v_0 r)) (subtypes A v_0)))))))
+(assert (forall ((A Int) (r Int) (T Int)) (let ((v_0 (ElementType_ T))) (=> (subtypes (NonNullRefArray A r) T) (or (subtypes System_dot_Array T) (and (= T (NonNullRefArray v_0 r)) (subtypes A v_0)))))))
+(assert (forall ((A Int) (r Int) (T Int)) (let ((v_0 (ValueArray A r))) (=> (subtypes v_0 T) (or (subtypes System_dot_Array T) (= T v_0))))))
+(assert (forall ((s Int) (f Int) (x Int)) (= (StructGet_ (StructSet_ s f x) f) x)))
+(assert (forall ((s Int) (f Int) (_f'_ Int) (x Int)) (=> (not (= f _f'_)) (= (StructGet_ (StructSet_ s f x) _f'_) (StructGet_ s _f'_)))))
+(assert (forall ((A Int) (B Int) (C Int)) (! (=> (subtypes C (AsDirectSubClass B A)) (= (OneClassDown C A) B)) :pattern ((subtypes C (AsDirectSubClass B A))) )))
+(assert (forall ((T Int)) (=> (= (IsValueType_ T) Smt_dot_true) (and (forall ((U Int)) (=> (subtypes T U) (= T U))) (forall ((U Int)) (=> (subtypes U T) (= T U)))))))
+(assert (subtypes System_dot_Type System_dot_Object))
+(assert (forall ((T Int)) (! (= (IsNotNull_ (TypeObject T) System_dot_Type) Smt_dot_true) :pattern ((TypeObject T)) )))
+(assert (forall ((T Int)) (! (= (TypeName (TypeObject T)) T) :pattern ((TypeObject T)) )))
+(assert (forall ((o Int) (T Int)) (! (= (= (Is_ o T) Smt_dot_true) (or (= o nullObject) (subtypes (typeof_ o) T))) :pattern ((Is_ o T)) )))
+(assert (forall ((o Int) (T Int)) (! (= (= (IsNotNull_ o T) Smt_dot_true) (and (not (= o nullObject)) (= (Is_ o T) Smt_dot_true))) :pattern ((IsNotNull_ o T)) )))
+(assert (forall ((o Int) (T Int)) (=> (= (Is_ o T) Smt_dot_true) (= (As_ o T) o))))
+(assert (forall ((o Int) (T Int)) (=> (not (= (Is_ o T) Smt_dot_true)) (= (As_ o T) nullObject))))
+(assert (forall ((h Int) (o Int)) (! (let ((v_0 (typeof_ o))) (=> (and (= (IsHeap h) Smt_dot_true) (not (= o nullObject)) (subtypes v_0 System_dot_Array)) (and (= (select2 h o inv_) v_0) (= (select2 h o localinv_) v_0)))) :pattern ((select2 h o inv_)) )))
+(assert (forall ((h Int) (o Int) (f Int)) (! (=> (and (= (IsHeap h) Smt_dot_true) (= (select2 h o allocated_) Smt_dot_true)) (= (IsAllocated h (select2 h o f)) Smt_dot_true)) :pattern ((IsAllocated h (select2 h o f))) )))
+(assert (forall ((h Int) (o Int) (f Int)) (! (=> (and (= (IsHeap h) Smt_dot_true) (= (select2 h o allocated_) Smt_dot_true)) (= (select2 h (select2 h o f) allocated_) Smt_dot_true)) :pattern ((select2 h (select2 h o f) allocated_)) )))
+(assert (forall ((h Int) (s Int) (f Int)) (! (=> (= (IsAllocated h s) Smt_dot_true) (= (IsAllocated h (StructGet_ s f)) Smt_dot_true)) :pattern ((IsAllocated h (StructGet_ s f))) )))
+(assert (forall ((h Int) (e Int) (i Int)) (! (=> (= (IsAllocated h e) Smt_dot_true) (= (IsAllocated h (RefArrayGet e i)) Smt_dot_true)) :pattern ((IsAllocated h (RefArrayGet e i))) )))
+(assert (forall ((h Int) (e Int) (i Int)) (! (=> (= (IsAllocated h e) Smt_dot_true) (= (IsAllocated h (ValueArrayGet e i)) Smt_dot_true)) :pattern ((IsAllocated h (ValueArrayGet e i))) )))
+(assert (forall ((h Int) (o Int)) (! (=> (= (IsAllocated h o) Smt_dot_true) (= (select2 h o allocated_) Smt_dot_true)) :pattern ((select2 h o allocated_)) )))
+(assert (forall ((h Int) (c Int)) (! (=> (= (IsHeap h) Smt_dot_true) (= (select2 h (ClassRepr c) allocated_) Smt_dot_true)) :pattern ((select2 h (ClassRepr c) allocated_)) )))
+(assert (forall ((f Int) (T Int)) (! (=> (= (AsNonNullRefField f T) f) (= (AsRefField f T) f)) :pattern ((AsNonNullRefField f T)) )))
+(assert (forall ((h Int) (o Int) (f Int) (T Int)) (! (=> (= (IsHeap h) Smt_dot_true) (= (Is_ (select2 h o (AsRefField f T)) T) Smt_dot_true)) :pattern ((select2 h o (AsRefField f T))) )))
+(assert (forall ((h Int) (o Int) (f Int) (T Int)) (! (=> (and (= (IsHeap h) Smt_dot_true) (not (= o nullObject)) (or (not (= o BeingConstructed_)) (= (= (select2 h BeingConstructed_ NonNullFieldsAreInitialized_) Smt_dot_true) true))) (not (= (select2 h o (AsNonNullRefField f T)) nullObject))) :pattern ((select2 h o (AsNonNullRefField f T))) )))
+(assert (forall ((h Int) (o Int) (f Int) (T Int)) (! (=> (= (IsHeap h) Smt_dot_true) (InRange (select2 h o (AsRangeField f T)) T)) :pattern ((select2 h o (AsRangeField f T))) )))
+(assert (forall ((o Int)) (! (not (= (IsMemberlessType_ (typeof_ o)) Smt_dot_true)) :pattern ((IsMemberlessType_ (typeof_ o))) )))
+(assert (not (= (IsImmutable_ System_dot_Object) Smt_dot_true)))
+(assert (forall ((T Int) (U Int)) (! (=> (subtypes U (AsImmutable_ T)) (and (= (IsImmutable_ U) Smt_dot_true) (= (AsImmutable_ U) U))) :pattern ((subtypes U (AsImmutable_ T))) )))
+(assert (forall ((T Int) (U Int)) (! (=> (subtypes U (AsMutable_ T)) (and (not (= (IsImmutable_ U) Smt_dot_true)) (= (AsMutable_ U) U))) :pattern ((subtypes U (AsMutable_ T))) )))
+(assert (forall ((o Int) (T Int)) (! (=> (and (not (= o nullObject)) (not (= o BeingConstructed_)) (subtypes (typeof_ o) (AsImmutable_ T))) (forall ((h Int)) (! (let ((v_0 (typeof_ o))) (=> (= (IsHeap h) Smt_dot_true) (and (= (select2 h o inv_) v_0) (= (select2 h o localinv_) v_0) (= (select2 h o ownerFrame_) PeerGroupPlaceholder_) (= (AsOwner o (select2 h o ownerRef_)) o) (forall ((t Int)) (! (=> (= (AsOwner o (select2 h t ownerRef_)) o) (or (= t o) (not (= (select2 h t ownerFrame_) PeerGroupPlaceholder_)))) :pattern ((AsOwner o (select2 h t ownerRef_))) ))))) :pattern ((IsHeap h)) ))) :pattern ((subtypes (typeof_ o) (AsImmutable_ T))) )))
+(assert (forall ((s Int)) (! (<= 0 (StringLength_ s)) :pattern ((StringLength_ s)) )))
+(assert (forall ((h Int) (o Int) (f Int) (T Int)) (! (let ((v_0 (select2 h o (AsRepField f T)))) (=> (and (= (IsHeap h) Smt_dot_true) (not (= v_0 nullObject))) (and (= (select2 h v_0 ownerRef_) o) (= (select2 h v_0 ownerFrame_) T)))) :pattern ((select2 h o (AsRepField f T))) )))
+(assert (forall ((h Int) (o Int) (f Int)) (! (let ((v_0 (select2 h o (AsPeerField f)))) (=> (and (= (IsHeap h) Smt_dot_true) (not (= v_0 nullObject))) (and (= (select2 h v_0 ownerRef_) (select2 h o ownerRef_)) (= (select2 h v_0 ownerFrame_) (select2 h o ownerFrame_))))) :pattern ((select2 h o (AsPeerField f))) )))
+(assert (forall ((h Int) (o Int)) (let ((v_0 (select2 h o ownerFrame_)) (v_1 (select2 h o ownerRef_)) (v_2 (typeof_ o))) (=> (and (= (IsHeap h) Smt_dot_true) (not (= v_0 PeerGroupPlaceholder_)) (subtypes (select2 h v_1 inv_) v_0) (not (= (select2 h v_1 localinv_) (BaseClass_ v_0)))) (and (= (select2 h o inv_) v_2) (= (select2 h o localinv_) v_2))))))
+(assert (forall ((o Int) (f Int) (h Int)) (! (let ((v_0 (select2 h o ownerFrame_)) (v_1 (select2 h o ownerRef_))) (=> (and (= (IsHeap h) Smt_dot_true) (not (= o nullObject)) (= (= (select2 h o allocated_) Smt_dot_true) true) (not (= v_0 PeerGroupPlaceholder_)) (subtypes (select2 h v_1 inv_) v_0) (not (= (select2 h v_1 localinv_) (BaseClass_ v_0)))) (= (select2 h o f) (FieldDependsOnFCO_ o f (select2 h (select2 h o FirstConsistentOwner_) exposeVersion_))))) :pattern ((select2 h (AsPureObject_ o) f)) )))
+(assert (forall ((o Int) (h Int)) (! (let ((v_0 (select2 h o ownerFrame_)) (v_1 (select2 h o ownerRef_)) (v_2 (select2 h o FirstConsistentOwner_))) (let ((v_3 (select2 h v_2 ownerFrame_)) (v_4 (select2 h v_2 ownerRef_))) (=> (and (= (IsHeap h) Smt_dot_true) (not (= o nullObject)) (= (= (select2 h o allocated_) Smt_dot_true) true) (not (= v_0 PeerGroupPlaceholder_)) (subtypes (select2 h v_1 inv_) v_0) (not (= (select2 h v_1 localinv_) (BaseClass_ v_0)))) (and (not (= v_2 nullObject)) (= (= (select2 h v_2 allocated_) Smt_dot_true) true) (or (= v_3 PeerGroupPlaceholder_) (not (subtypes (select2 h v_4 inv_) v_3)) (= (select2 h v_4 localinv_) (BaseClass_ v_3))))))) :pattern ((select2 h o FirstConsistentOwner_)) )))
+(assert (forall ((x Int) (p Int)) (! (= (Unbox (Box x p)) x) :pattern ((Unbox (Box x p))) )))
+(assert (forall ((p Int)) (! (=> (= (IsValueType_ (UnboxedType p)) Smt_dot_true) (forall ((heap Int) (x Int)) (let ((v_0 (Box x p))) (let ((v_1 (typeof_ v_0))) (=> (= (IsHeap heap) Smt_dot_true) (and (= (select2 heap v_0 inv_) v_1) (= (select2 heap v_0 localinv_) v_1))))))) :pattern ((IsValueType_ (UnboxedType p))) )))
+(assert (forall ((x Int) (p Int)) (let ((v_0 (Box x p))) (=> (and (subtypes (UnboxedType v_0) System_dot_Object) (= v_0 p)) (= x p)))))
+(assert (forall ((p Int) (typ Int)) (! (= (= (UnboxedType p) typ) (not (= (BoxTester p typ) nullObject))) :pattern ((BoxTester p typ)) )))
+(assert (= (IsValueType_ System_dot_SByte) Smt_dot_true))
+(assert (= (IsValueType_ System_dot_Byte) Smt_dot_true))
+(assert (= (IsValueType_ System_dot_Int16) Smt_dot_true))
+(assert (= (IsValueType_ System_dot_UInt16) Smt_dot_true))
+(assert (= (IsValueType_ System_dot_Int32) Smt_dot_true))
+(assert (= (IsValueType_ System_dot_UInt32) Smt_dot_true))
+(assert (= (IsValueType_ System_dot_Int64) Smt_dot_true))
+(assert (= (IsValueType_ System_dot_UInt64) Smt_dot_true))
+(assert (= (IsValueType_ System_dot_Char) Smt_dot_true))
+(assert (< int_m9223372036854775808 int_m2147483648))
+(assert (< int_m2147483648 (- 0 100000)))
+(assert (< 100000 int_2147483647))
+(assert (< int_2147483647 int_4294967295))
+(assert (< int_4294967295 int_9223372036854775807))
+(assert (< int_9223372036854775807 int_18446744073709551615))
+(assert (forall ((i Int)) (= (InRange i System_dot_SByte) (and (<= (- 0 128) i) (< i 128)))))
+(assert (forall ((i Int)) (= (InRange i System_dot_Byte) (and (<= 0 i) (< i 256)))))
+(assert (forall ((i Int)) (= (InRange i System_dot_Int16) (and (<= (- 0 32768) i) (< i 32768)))))
+(assert (forall ((i Int)) (= (InRange i System_dot_UInt16) (and (<= 0 i) (< i 65536)))))
+(assert (forall ((i Int)) (= (InRange i System_dot_Int32) (and (<= int_m2147483648 i) (<= i int_2147483647)))))
+(assert (forall ((i Int)) (= (InRange i System_dot_UInt32) (and (<= 0 i) (<= i int_4294967295)))))
+(assert (forall ((i Int)) (= (InRange i System_dot_Int64) (and (<= int_m9223372036854775808 i) (<= i int_9223372036854775807)))))
+(assert (forall ((i Int)) (= (InRange i System_dot_UInt64) (and (<= 0 i) (<= i int_18446744073709551615)))))
+(assert (forall ((i Int)) (= (InRange i System_dot_Char) (and (<= 0 i) (< i 65536)))))
+(assert (forall ((b Int) (x Int) (y Int)) (! (=> (= b Smt_dot_true) (= (IfThenElse_ b x y) x)) :pattern ((IfThenElse_ b x y)) )))
+(assert (forall ((b Int) (x Int) (y Int)) (! (=> (not (= b Smt_dot_true)) (= (IfThenElse_ b x y) y)) :pattern ((IfThenElse_ b x y)) )))
+(assert (forall ((x Int) (y Int)) (! (= (modulo x y) (- x (multiply (divide x y) y))) :pattern ((modulo x y))  :pattern ((divide x y)) )))
+(assert (forall ((x Int) (y Int)) (! (let ((v_0 (modulo x y))) (=> (and (<= 0 x) (< 0 y)) (and (<= 0 v_0) (< v_0 y)))) :pattern ((modulo x y)) )))
+(assert (forall ((x Int) (y Int)) (! (let ((v_0 (modulo x y))) (=> (and (<= 0 x) (< y 0)) (and (<= 0 v_0) (< v_0 (- 0 y))))) :pattern ((modulo x y)) )))
+(assert (forall ((x Int) (y Int)) (! (let ((v_0 (modulo x y))) (=> (and (<= x 0) (< 0 y)) (and (< (- 0 y) v_0) (<= v_0 0)))) :pattern ((modulo x y)) )))
+(assert (forall ((x Int) (y Int)) (! (let ((v_0 (modulo x y))) (=> (and (<= x 0) (< y 0)) (and (< y v_0) (<= v_0 0)))) :pattern ((modulo x y)) )))
+(assert (forall ((x Int) (y Int)) (=> (and (<= 0 x) (<= 0 y)) (= (modulo (+ x y) y) (modulo x y)))))
+(assert (forall ((x Int) (y Int)) (=> (and (<= 0 x) (<= 0 y)) (= (modulo (+ y x) y) (modulo x y)))))
+(assert (forall ((x Int) (y Int)) (let ((v_0 (- x y))) (=> (and (<= 0 v_0) (<= 0 y)) (= (modulo v_0 y) (modulo x y))))))
+(assert (forall ((a Int) (b Int) (d Int)) (! (=> (and (<= 2 d) (= (modulo a d) (modulo b d)) (< a b)) (<= (+ a d) b)) :pattern ((modulo a d) (modulo b d)) )))
+(assert (forall ((x Int) (y Int)) (! (=> (or (<= 0 x) (<= 0 y)) (<= 0 (and_ x y))) :pattern ((and_ x y)) )))
+(assert (forall ((x Int) (y Int)) (! (let ((v_0 (or_ x y))) (=> (and (<= 0 x) (<= 0 y)) (and (<= 0 v_0) (<= v_0 (+ x y))))) :pattern ((or_ x y)) )))
+(assert (forall ((i Int)) (! (= (shl_ i 0) i) :pattern ((shl_ i 0)) )))
+(assert (forall ((i Int) (j Int)) (=> (<= 0 j) (= (shl_ i (+ j 1)) ( * (shl_ i j) 2)))))
+(assert (forall ((i Int)) (! (= (shr_ i 0) i) :pattern ((shr_ i 0)) )))
+(assert (forall ((i Int) (j Int)) (=> (<= 0 j) (= (shr_ i (+ j 1)) (divide (shr_ i j) 2)))))
+(assert (forall ((a Int) (b Int)) (! (= (= (System_dot_String_dot_Equals_System_dot_String_ a b) Smt_dot_true) (= (System_dot_String_dot_Equals_System_dot_String_System_dot_String_ a b) Smt_dot_true)) :pattern ((System_dot_String_dot_Equals_System_dot_String_ a b)) )))
+(assert (forall ((a Int) (b Int)) (! (= (= (System_dot_String_dot_Equals_System_dot_String_System_dot_String_ a b) Smt_dot_true) (= (System_dot_String_dot_Equals_System_dot_String_System_dot_String_ b a) Smt_dot_true)) :pattern ((System_dot_String_dot_Equals_System_dot_String_System_dot_String_ a b)) )))
+(assert (forall ((a Int) (b Int)) (! (=> (and (not (= a nullObject)) (not (= b nullObject)) (= (System_dot_String_dot_Equals_System_dot_String_System_dot_String_ a b) Smt_dot_true)) (= (System_dot_String_dot_IsInterned_System_dot_String_notnull_ a) (System_dot_String_dot_IsInterned_System_dot_String_notnull_ b))) :pattern ((System_dot_String_dot_Equals_System_dot_String_System_dot_String_ a b)) )))
+(assert (not (= (IsStaticField Bag_dot_n) Smt_dot_true)))
+(assert (= (IsDirectlyModifiableField Bag_dot_n) Smt_dot_true))
+(assert (= (DeclType Bag_dot_n) Bag))
+(assert (= (AsRangeField Bag_dot_n System_dot_Int32) Bag_dot_n))
+(assert (not (= (IsStaticField Bag_dot_a) Smt_dot_true)))
+(assert (= (IsDirectlyModifiableField Bag_dot_a) Smt_dot_true))
+(assert (= (AsRepField Bag_dot_a Bag) Bag_dot_a))
+(assert (= (DeclType Bag_dot_a) Bag))
+(assert (= (AsNonNullRefField Bag_dot_a (ValueArray System_dot_Int32 1)) Bag_dot_a))
+(assert (subtypes Bag Bag))
+(assert (= (BaseClass_ Bag) System_dot_Object))
+(assert (subtypes Bag (BaseClass_ Bag)))
+(assert (= (AsDirectSubClass Bag (BaseClass_ Bag)) Bag))
+(assert (not (= (IsImmutable_ Bag) Smt_dot_true)))
+(assert (= (AsMutable_ Bag) Bag))
+(assert (forall ((oi_ Int) (h_ Int)) (! (let ((v_0 (select2 h_ oi_ Bag_dot_n))) (=> (and (= (IsHeap h_) Smt_dot_true) (subtypes (select2 h_ oi_ inv_) Bag) (not (= (select2 h_ oi_ localinv_) System_dot_Object))) (and (<= 0 v_0) (<= v_0 (Length_ (select2 h_ oi_ Bag_dot_a)))))) :pattern ((subtypes (select2 h_ oi_ inv_) Bag)) )))
+(assert (forall ((U_ Int)) (! (=> (subtypes U_ System_dot_Boolean) (= U_ System_dot_Boolean)) :pattern ((subtypes U_ System_dot_Boolean)) )))
+(assert (subtypes Microsoft_dot_Contracts_dot_ObjectInvariantException Microsoft_dot_Contracts_dot_ObjectInvariantException))
+(assert (subtypes Microsoft_dot_Contracts_dot_GuardException Microsoft_dot_Contracts_dot_GuardException))
+(assert (subtypes System_dot_Exception System_dot_Exception))
+(assert (= (BaseClass_ System_dot_Exception) System_dot_Object))
+(assert (subtypes System_dot_Exception (BaseClass_ System_dot_Exception)))
+(assert (= (AsDirectSubClass System_dot_Exception (BaseClass_ System_dot_Exception)) System_dot_Exception))
+(assert (not (= (IsImmutable_ System_dot_Exception) Smt_dot_true)))
+(assert (= (AsMutable_ System_dot_Exception) System_dot_Exception))
+(assert (subtypes System_dot_Runtime_dot_Serialization_dot_ISerializable System_dot_Object))
+(assert (= (IsMemberlessType_ System_dot_Runtime_dot_Serialization_dot_ISerializable) Smt_dot_true))
+(assert (subtypes System_dot_Exception System_dot_Runtime_dot_Serialization_dot_ISerializable))
+(assert (subtypes System_dot_Runtime_dot_InteropServices_dot__Exception System_dot_Object))
+(assert (= (IsMemberlessType_ System_dot_Runtime_dot_InteropServices_dot__Exception) Smt_dot_true))
+(assert (subtypes System_dot_Exception System_dot_Runtime_dot_InteropServices_dot__Exception))
+(assert (= (BaseClass_ Microsoft_dot_Contracts_dot_GuardException) System_dot_Exception))
+(assert (subtypes Microsoft_dot_Contracts_dot_GuardException (BaseClass_ Microsoft_dot_Contracts_dot_GuardException)))
+(assert (= (AsDirectSubClass Microsoft_dot_Contracts_dot_GuardException (BaseClass_ Microsoft_dot_Contracts_dot_GuardException)) Microsoft_dot_Contracts_dot_GuardException))
+(assert (not (= (IsImmutable_ Microsoft_dot_Contracts_dot_GuardException) Smt_dot_true)))
+(assert (= (AsMutable_ Microsoft_dot_Contracts_dot_GuardException) Microsoft_dot_Contracts_dot_GuardException))
+(assert (= (BaseClass_ Microsoft_dot_Contracts_dot_ObjectInvariantException) Microsoft_dot_Contracts_dot_GuardException))
+(assert (subtypes Microsoft_dot_Contracts_dot_ObjectInvariantException (BaseClass_ Microsoft_dot_Contracts_dot_ObjectInvariantException)))
+(assert (= (AsDirectSubClass Microsoft_dot_Contracts_dot_ObjectInvariantException (BaseClass_ Microsoft_dot_Contracts_dot_ObjectInvariantException)) Microsoft_dot_Contracts_dot_ObjectInvariantException))
+(assert (not (= (IsImmutable_ Microsoft_dot_Contracts_dot_ObjectInvariantException) Smt_dot_true)))
+(assert (= (AsMutable_ Microsoft_dot_Contracts_dot_ObjectInvariantException) Microsoft_dot_Contracts_dot_ObjectInvariantException))
+(assert (subtypes System_dot_Array System_dot_Array))
+(assert (= (BaseClass_ System_dot_Array) System_dot_Object))
+(assert (subtypes System_dot_Array (BaseClass_ System_dot_Array)))
+(assert (= (AsDirectSubClass System_dot_Array (BaseClass_ System_dot_Array)) System_dot_Array))
+(assert (not (= (IsImmutable_ System_dot_Array) Smt_dot_true)))
+(assert (= (AsMutable_ System_dot_Array) System_dot_Array))
+(assert (subtypes System_dot_ICloneable System_dot_Object))
+(assert (= (IsMemberlessType_ System_dot_ICloneable) Smt_dot_true))
+(assert (subtypes System_dot_Array System_dot_ICloneable))
+(assert (subtypes System_dot_Collections_dot_IList System_dot_Object))
+(assert (subtypes System_dot_Collections_dot_ICollection System_dot_Object))
+(assert (subtypes System_dot_Collections_dot_IEnumerable System_dot_Object))
+(assert (= (IsMemberlessType_ System_dot_Collections_dot_IEnumerable) Smt_dot_true))
+(assert (subtypes System_dot_Collections_dot_ICollection System_dot_Collections_dot_IEnumerable))
+(assert (= (IsMemberlessType_ System_dot_Collections_dot_ICollection) Smt_dot_true))
+(assert (subtypes System_dot_Collections_dot_IList System_dot_Collections_dot_ICollection))
+(assert (subtypes System_dot_Collections_dot_IList System_dot_Collections_dot_IEnumerable))
+(assert (= (IsMemberlessType_ System_dot_Collections_dot_IList) Smt_dot_true))
+(assert (subtypes System_dot_Array System_dot_Collections_dot_IList))
+(assert (subtypes System_dot_Array System_dot_Collections_dot_ICollection))
+(assert (subtypes System_dot_Array System_dot_Collections_dot_IEnumerable))
+(assert (= (IsMemberlessType_ System_dot_Array) Smt_dot_true))
+(assert (subtypes System_dot_Type System_dot_Type))
+(assert (subtypes System_dot_Reflection_dot_MemberInfo System_dot_Reflection_dot_MemberInfo))
+(assert (= (BaseClass_ System_dot_Reflection_dot_MemberInfo) System_dot_Object))
+(assert (subtypes System_dot_Reflection_dot_MemberInfo (BaseClass_ System_dot_Reflection_dot_MemberInfo)))
+(assert (= (AsDirectSubClass System_dot_Reflection_dot_MemberInfo (BaseClass_ System_dot_Reflection_dot_MemberInfo)) System_dot_Reflection_dot_MemberInfo))
+(assert (= (IsImmutable_ System_dot_Reflection_dot_MemberInfo) Smt_dot_true))
+(assert (= (AsImmutable_ System_dot_Reflection_dot_MemberInfo) System_dot_Reflection_dot_MemberInfo))
+(assert (subtypes System_dot_Reflection_dot_ICustomAttributeProvider System_dot_Object))
+(assert (= (IsMemberlessType_ System_dot_Reflection_dot_ICustomAttributeProvider) Smt_dot_true))
+(assert (subtypes System_dot_Reflection_dot_MemberInfo System_dot_Reflection_dot_ICustomAttributeProvider))
+(assert (subtypes System_dot_Runtime_dot_InteropServices_dot__MemberInfo System_dot_Object))
+(assert (= (IsMemberlessType_ System_dot_Runtime_dot_InteropServices_dot__MemberInfo) Smt_dot_true))
+(assert (subtypes System_dot_Reflection_dot_MemberInfo System_dot_Runtime_dot_InteropServices_dot__MemberInfo))
+(assert (= (IsMemberlessType_ System_dot_Reflection_dot_MemberInfo) Smt_dot_true))
+(assert (= (BaseClass_ System_dot_Type) System_dot_Reflection_dot_MemberInfo))
+(assert (subtypes System_dot_Type (BaseClass_ System_dot_Type)))
+(assert (= (AsDirectSubClass System_dot_Type (BaseClass_ System_dot_Type)) System_dot_Type))
+(assert (= (IsImmutable_ System_dot_Type) Smt_dot_true))
+(assert (= (AsImmutable_ System_dot_Type) System_dot_Type))
+(assert (subtypes System_dot_Runtime_dot_InteropServices_dot__Type System_dot_Object))
+(assert (= (IsMemberlessType_ System_dot_Runtime_dot_InteropServices_dot__Type) Smt_dot_true))
+(assert (subtypes System_dot_Type System_dot_Runtime_dot_InteropServices_dot__Type))
+(assert (subtypes System_dot_Reflection_dot_IReflect System_dot_Object))
+(assert (= (IsMemberlessType_ System_dot_Reflection_dot_IReflect) Smt_dot_true))
+(assert (subtypes System_dot_Type System_dot_Reflection_dot_IReflect))
+(assert (= (IsMemberlessType_ System_dot_Type) Smt_dot_true))
+(assert (subtypes Microsoft_dot_Contracts_dot_ICheckedException System_dot_Object))
+(assert (= (IsMemberlessType_ Microsoft_dot_Contracts_dot_ICheckedException) Smt_dot_true))
+(assert (forall ((A Int) (i Int) (v Int)) (= (select1 (store1 A i v) i) v)))
+(assert (forall ((A Int) (i Int) (j Int) (v Int)) (=> (not (= i j)) (= (select1 (store1 A i v) j) (select1 A j)))))
+(assert (forall ((A Int) (o Int) (f Int) (v Int)) (= (select2 (store2 A o f v) o f) v)))
+(assert (forall ((A Int) (o Int) (f Int) (p Int) (g Int) (v Int)) (=> (not (= o p)) (= (select2 (store2 A o f v) p g) (select2 A p g)))))
+(assert (forall ((A Int) (o Int) (f Int) (p Int) (g Int) (v Int)) (=> (not (= f g)) (= (select2 (store2 A o f v) p g) (select2 A p g)))))
+(assert (forall ((x Int) (y Int)) (= (= (boolIff x y) Smt_dot_true) (= (= x Smt_dot_true) (= y Smt_dot_true)))))
+(assert (forall ((x Int) (y Int)) (= (= (boolImplies x y) Smt_dot_true) (=> (= x Smt_dot_true) (= y Smt_dot_true)))))
+(assert (forall ((x Int) (y Int)) (= (= (boolAnd x y) Smt_dot_true) (and (= x Smt_dot_true) (= y Smt_dot_true)))))
+(assert (forall ((x Int) (y Int)) (= (= (boolOr x y) Smt_dot_true) (or (= x Smt_dot_true) (= y Smt_dot_true)))))
+(assert (forall ((x Int)) (! (= (= (boolNot x) Smt_dot_true) (not (= x Smt_dot_true))) :pattern ((boolNot x)) )))
+(assert (forall ((x Int) (y Int)) (= (= (anyEqual x y) Smt_dot_true) (= x y))))
+(assert (forall ((x Int) (y Int)) (! (= (= (anyNeq x y) Smt_dot_true) (not (= x y))) :pattern ((anyNeq x y)) )))
+(assert (forall ((x Int) (y Int)) (= (= (intLess x y) Smt_dot_true) (< x y))))
+(assert (forall ((x Int) (y Int)) (= (= (intAtMost x y) Smt_dot_true) (<= x y))))
+(assert (forall ((x Int) (y Int)) (= (= (intAtLeast x y) Smt_dot_true) (>= x y))))
+(assert (forall ((x Int) (y Int)) (= (= (intGreater x y) Smt_dot_true) (> x y))))
+(assert (distinct Smt_dot_false Smt_dot_true))
+(assert (forall ((t Int)) (! (subtypes t t) :pattern ((subtypes t t)) )))
+(assert (forall ((t Int) (u Int) (v Int)) (! (=> (and (subtypes t u) (subtypes u v)) (subtypes t v)) :pattern ((subtypes t u) (subtypes u v)) )))
+(assert (forall ((t Int) (u Int)) (! (=> (and (subtypes t u) (subtypes u t)) (= t u)) :pattern ((subtypes t u) (subtypes u t)) )))
+(assert (let ((v_0 (forall ((o_ Int)) (let ((v_5 (select2 Heap_ o_ ownerRef_)) (v_6 (select2 Heap_ o_ ownerFrame_))) (=> (and (not (= o_ nullObject)) (= (= (select2 Heap_ o_ allocated_) Smt_dot_true) true)) (and (= v_5 v_5) (= v_6 v_6)))))) (v_1 (= ReallyLastGeneratedExit_correct Smt_dot_true)) (v_2 (= block6086_correct Smt_dot_true)) (v_3 (= block6069_correct Smt_dot_true)) (v_4 (= entry_correct Smt_dot_true))) (not (=> (=> (=> true (=> (= (IsHeap Heap_) Smt_dot_true) (=> (= BeingConstructed_ nullObject) (=> true (=> true (=> (=> (=> true (=> true (=> true (=> (=> (=> true (=> true (=> true (=> (=> (=> true (and v_0 (=> v_0 (=> true true)))) v_1) v_1)))) v_2) v_2)))) v_3) v_3)))))) v_4) v_4))))
+(check-sat)
+.
+  intros.
+  cbv beta delta [with_pattern] in *.
+
+
 (* https://www.starexec.org/starexec/secure/details/benchmark.jsp?id=6920515
 (amortized queues in leon) declares datatypes, and these cannot be parsed as a goal
-
-UFLIA example from boogie from SMT competition
-
-https://www.starexec.org/starexec/services/benchmarks/7158337/contents?limit=-1
-
 *)
